refactoring `split_bytes` for easier proofs

coq/CheriMemory/CheriMorelloMemory.v
@@ -1117,6 +1117,28 @@ Module Type CheriMemoryImpl
     | PV prov ptrval => (prov,ptrval)
     end.
 
+
+  (* Part of [split_bytes] definition factored out to simplify proofs *)
+  Definition split_bytes_fold (bs : list AbsByte) (p0:provenance)
+    : serr ((option provenance) * list (option ascii) * option nat)
+    :=
+    monadic_fold_left
+      (fun '(prov_acc_maybe, val_acc, offset_acc_maybe) b =>
+         prov_acc' <-
+           match prov_acc_maybe, b.(prov) with
+           | Some p1, p2 =>
+               if provenance_eqb p1 p2 then ret prov_acc_maybe else ret None
+           (* once invalid stays always invalid *)
+           | None, _ => ret None
+           end ;;
+         let offset_acc' :=
+           match offset_acc_maybe, b.(copy_offset) with
+           | Some n1, Some n2 =>
+               if Nat.eqb n1 n2 then Some (S n1) else None
+           | _, _ => None
+           end in
+         ret (prov_acc', b.(value)::val_acc, offset_acc')) bs ((Some p0, [], Some O)).
+
   (* Given a (non-empty) list of bytes combine their provenance (if
      compatible). Returns the empty provenance otherwise *)
   Definition split_bytes (bs : list AbsByte)
@@ -1125,24 +1147,7 @@ Module Type CheriMemoryImpl
     | [] => raise "AbsByte.split_bytes: called on an empty list"
     | b::bs' =>
         '(prov_maybe, rev_values, offset_status_maybe) <-
-          monadic_fold_left
-            (fun '(prov_acc_maybe, val_acc, offset_acc_maybe) b =>
-               prov_acc' <-
-                 match prov_acc_maybe, b.(prov) with
-                 | Some p1, p2 =>
-                     if provenance_eqb p1 p2 then ret prov_acc_maybe else ret None
-                 (* once invalid stays always invalid *)
-                 | None, _ => ret None
-                 end ;;
-               let offset_acc' :=
-                 match offset_acc_maybe, b.(copy_offset) with
-                 | Some n1, Some n2 =>
-                     if Nat.eqb n1 n2 then Some (S n1) else None
-                 | _, _ => None
-                 end in
-               ret (prov_acc', b.(value)::val_acc, offset_acc'))
-            (b::bs') ((Some b.(prov), [], Some O)) ;;
-
+          split_bytes_fold bs b.(prov);;
         let values := List.rev rev_values in
         ret (opt_def (PNVI_prov Prov_none) prov_maybe ,
             is_some offset_status_maybe && is_some prov_maybe,
